Fix find proof to work with new wf_context

src/Tree_stack.thy
@@ -34,14 +34,6 @@ fun linked_context :: "(left_bound * (node_t * nat) * right_bound) => context_t 
 "linked_context (lb,ni,rb) ((plb,pi,prb)#pis) = (
   is_subnode ni pi & linked_context (plb,pi,prb) pis)"
 
-definition wellformed_context_1 :: "rmbs_t => (left_bound * (node_t * nat) * right_bound) => bool " where
-"wellformed_context_1 rmbs lbnirb == (
-let (lb,((l,cs),i),rb) = lbnirb in
-let node = (Node(l,cs)) in(
-wellformed_tree rmbs node
-& i : (subtree_indexes (l,cs)))
-& check_keys lb (keys node) rb)"
-
 definition get_lower_upper_keys_for_node_t :: "key list => left_bound => nat => right_bound => (key option * key option)" where
 "get_lower_upper_keys_for_node_t ls lb i rb == (
 let l = if (i = 0) then lb else Some(ls ! (i - 1))     in
@@ -49,15 +41,34 @@ let u = if (i = (length ls)) then rb else Some(ls ! i) in
 (l,u)
 )"
 
+definition wellformed_context_1 :: "rmbs_t => (left_bound * (node_t * nat) * right_bound) => bool " where
+"wellformed_context_1 rmbs lbnirb == (
+let (lb,((ls,cs),i),rb) = lbnirb in
+let (l,u) = get_lower_upper_keys_for_node_t ls lb i rb  in
+let node = (Node(ls,cs)) in
+wellformed_tree rmbs node
+& i : (subtree_indexes (ls,cs))
+& check_keys lb (keys (cs!i)) rb)"
+
 fun wellformed_context :: "context_t => bool" where
 "wellformed_context Nil = True" |
-"wellformed_context (x # Nil) = wellformed_context_1 (Rmbs True) x" |
+"wellformed_context ((lb,((ls,rs),i),rb) # Nil) =
+(
+let (l,u) = get_lower_upper_keys_for_node_t ls lb i rb  in
+(if i = 0 then lb = None else lb = l)
+&
+(if i = length ls then rb = None else rb = u)
+&
+wellformed_context_1 (Rmbs True) (lb,((ls,rs),i),rb))" |
 "wellformed_context (x1 # (x2 # rest)) = (
-let (lb,((ls,_),i),rb) = x2 in
-let (l2,u2) = get_lower_upper_keys_for_node_t ls lb i rb in
-let (l1,_,u1) = x1 in
+let (lb,((ls,_),i),rb) = x1 in
+let (lb',_,rb') = x2 in
 wellformed_context_1 (Rmbs False) x1
-& (l1,u1) = (l2,u2)
+& 
+(let (l,u) = get_lower_upper_keys_for_node_t ls lb i rb  in
+ (if i = 0 then lb = lb' else lb = l)
+ & (if i = (length ls) then rb = rb' else rb = u)
+)
 & linked_context x1 (x2#rest)
 & wellformed_context (x2#rest)
 )
