src/Find_proof.thy
@@ -1,5 +1,5 @@
 theory Find_proof
-imports Find_tree_stack
+imports Key_lt_order Find_tree_stack
 begin
 
 definition invariant_wf_fts :: "bool" where
@@ -14,6 +14,12 @@ case fts' of None => True
 
 lemma set_butlast_lessThan:"set (butlast [0..<n]) = {0..<n -1}"
 apply (case_tac n,force+)
+done
+
+lemma keys_Cons: 
+"keys (Node (l, cs)) = l@((List.map keys cs) |> List.concat)"
+apply (simp add:keys_def rev_apply_def keys_1_def)
+apply (induct cs) apply (force simp add:keys_def rev_apply_def)+
 done
 
 lemma invariant_wf_fts: "invariant_wf_fts"
@@ -69,26 +75,173 @@ prefer 2
   apply (subgoal_tac "keys_ordered child") prefer 2 apply (force simp add:keys_ordered_def forall_subtrees_def rev_apply_def list_all_iff)
   apply force
  apply simp
+ apply (subgoal_tac "ks ~= []") prefer 2 apply (simp add:wellformed_fts_focus_def wellformed_tree_def wf_size_def,case_tac ctx,force,force simp add:forall_subtrees_def rev_apply_def wf_size_1_def Let_def)
+ apply (subgoal_tac "wellformed_fts_1 (Fts_state (k, child, (l, ((ks, rs), index), u) # ctx))")
+ prefer 2
+  apply (simp add:dest_fts_state_def wellformed_fts_1_def)
+  apply (simp add:get_lower_upper_keys_for_node_t_def check_keys_def)
+  apply (subgoal_tac "index < length ks --> key_lt k (ks ! index)")
+  prefer 2
+   apply rule
+   apply (simp add:search_key_to_index_def Let_def)
+   apply (case_tac "List.find (\<lambda>x. key_lt k (ks ! x)) [0..<length ks]",force)
+   apply (simp add:find_Some_iff)
+   apply (erule exE)+
+   apply force
+  apply (subgoal_tac "0 < index --> key_le (ks ! (index - Suc 0)) k")
+  prefer 2
+   apply rule
+   apply (simp add:search_key_to_index_def Let_def)
+   apply (subgoal_tac "total_order_key_lte") prefer 2 apply (force intro:FIXME) (*move in assumptions*)
+   apply (case_tac "List.find (\<lambda>x. key_lt k (ks ! x)) [0..<length ks]")
+    (*None*)
+    apply (simp add:find_None_iff)
+    apply (drule_tac x="index-1" in spec)
+    apply (force simp add:neg_key_lt)
+    
+    (*Some*)
+    apply (simp add:find_Some_iff)
+    apply (erule exE)+
+    apply (erule conjE)+
+    apply (drule_tac x="index-1" in spec)
+    apply (force simp add:neg_key_lt)
+    
+  apply (case_tac "index = 0")
+   apply (case_tac ctx,force,simp)
+   apply (case_tac list)
+    apply clarsimp
+    apply (case_tac x,simp add:get_lower_upper_keys_for_node_t_def Let_def,case_tac ba,force,force)
+    apply (simp add:get_lower_upper_keys_for_node_t_def Let_def check_keys_def)
+    apply (simp add:wellformed_context_1_def check_keys_def )
+    apply clarsimp
+    apply (case_tac l,force)
+    apply (case_tac "ba = 0",force,force)
+   
+    (*list ~= []*)
+    apply clarsimp
+    apply (case_tac l,force)
+    apply (rename_tac kl)
+    apply (simp add:get_lower_upper_keys_for_node_t_def Let_def check_keys_def)
+    apply (case_tac ba,force)
+    apply force
+   (*index = length ks*)
+   apply simp
+   apply (case_tac u,force)
+   apply (rename_tac kr)
+   apply (case_tac ctx,force,simp)
+   apply (case_tac list)
+    apply clarsimp
+    apply (simp add:get_lower_upper_keys_for_node_t_def Let_def check_keys_def)
+    apply (simp add:wellformed_context_1_def check_keys_def )
+    apply clarsimp
+    apply (case_tac "ba = length aa",force,force)
+   
+    (*list ~= []*)
+    apply clarsimp
+    apply (rename_tac kl)
+    apply (simp add:get_lower_upper_keys_for_node_t_def Let_def check_keys_def)
+    apply (case_tac "ba=length aa",force)
+    apply force
  apply (case_tac ctx)
  (*ctx = [] *)
+ apply simp
  apply (simp add:wellformed_context_1_def Let_def wellformed_fts_focus_def subtree_indexes_def check_keys_def get_lower_upper_keys_for_node_t_def)
  apply rule
   apply (case_tac l) apply force
+  apply (rename_tac im1ks)
   apply simp
-  apply (subgoal_tac "a = (ks ! (index - 1))") prefer 2 apply (metis option.distinct(1) option.inject)
+  apply (subgoal_tac "im1ks = (ks ! (index - 1))") prefer 2 apply (metis option.distinct(1) option.inject)
   apply simp
   apply (simp add:wellformed_tree_def keys_ordered_def forall_subtrees_def rev_apply_def keys_ordered_1_def key_indexes_def set_butlast_lessThan atLeast0LessThan lessThan_def check_keys_def)
-  apply (simp add:keys_def rev_apply_def keys_1_def)
-  (*ERROR IN DEFINITIONS*)
-  apply (fast intro:FIXME)
+  apply (simp add:keys_consistent_def forall_subtrees_def rev_apply_def keys_consistent_1_def check_keys_def key_indexes_def atLeast0LessThan lessThan_def)
+  apply (erule conjE)+
+  apply (drule_tac x="index - Suc 0" in spec) back
+  apply force
 
-  apply (case_tac u) apply (force simp add:dest_fts_state_def wellformed_fts_1_def)
-  apply (fast intro:FIXME)
+  apply (case_tac u) apply (force)
+  apply (rename_tac iks)
+  apply simp
+  apply (subgoal_tac "iks = ks ! index") prefer 2 apply (case_tac "index = length ks",force,force)
+  apply simp
+  apply (simp add:wellformed_tree_def keys_ordered_def forall_subtrees_def rev_apply_def keys_ordered_1_def key_indexes_def set_butlast_lessThan atLeast0LessThan lessThan_def check_keys_def)
+  apply (simp add:keys_consistent_def forall_subtrees_def rev_apply_def keys_consistent_1_def check_keys_def key_indexes_def atLeast0LessThan lessThan_def)
+  apply (erule conjE)+
+  apply (drule_tac x="index" in spec)
+  apply force
 
   (*ctx = a#list*)
   apply simp
-  apply (fast intro:FIXME)
+  apply rule
+   (*wellformed_context_1*)
+   apply (simp add:wellformed_context_1_def wellformed_fts_focus_def)
+   apply (simp add:subtree_indexes_def)
+   apply (simp add:check_keys_def)
+   apply (simp add:get_lower_upper_keys_for_node_t_def)
+   apply (case_tac a,simp)
+   apply (erule conjE)+
+   apply (subgoal_tac "wellformed_context_1 (Rmbs (list = [])) (lb, b, rb)") prefer 2 apply (case_tac list, force,force) 
+   apply (rule)
+    (*case l of None \<Rightarrow> True | Some kl \<Rightarrow> Ball (set (keys child)) (key_le kl)*)
+    apply (case_tac l,force)
+    apply (rename_tac kl)
+    apply (simp add:wellformed_context_1_def,case_tac b,case_tac ab,simp)
+    apply (case_tac "index = 0")
+     apply (simp add:check_keys_def wellformed_fts_1_def dest_fts_state_def)
+     apply (erule conjE)+
+     apply (drule_tac t="bb!ba" in sym) back
+     apply (simp add:keys_def rev_apply_def keys_1_def)
+     apply blast
 
- (*apply (force simp add:dest_fts_state_def wellformed_fts_1_def)*)
+     (*index ~= 0*)
+     apply simp
+     apply (drule_tac t="kl" in sym)
+     apply simp
+     apply (simp add:wellformed_tree_def keys_ordered_def forall_subtrees_def rev_apply_def keys_ordered_1_def key_indexes_def set_butlast_lessThan atLeast0LessThan lessThan_def check_keys_def)
+     apply (force simp add:keys_consistent_def forall_subtrees_def rev_apply_def keys_consistent_1_def check_keys_def key_indexes_def atLeast0LessThan lessThan_def)
+    
+    (*case u of None \<Rightarrow> True | Some kr \<Rightarrow> \<forall>k\<in>set (keys child). key_lt k kr*)
+    apply (case_tac u,force)
+    
+    (*u = Some kr*)
+    apply (rename_tac kr)
+    apply (simp add:wellformed_context_1_def,case_tac b,case_tac ab,simp)
+    apply (case_tac "index = length ks")
+     (*index = length ks*)
+     apply (simp add:check_keys_def wellformed_fts_1_def dest_fts_state_def)
+     apply (erule conjE)+
+     apply (drule_tac t="bb!ba" in sym) back
+     apply (simp add:keys_def rev_apply_def keys_1_def)
+     apply blast
+
+     (*index ~= length ks*)
+     apply simp
+     apply (drule_tac t="kr" in sym)
+     apply simp
+     apply (simp add:wellformed_tree_def keys_ordered_def forall_subtrees_def rev_apply_def keys_ordered_1_def key_indexes_def set_butlast_lessThan atLeast0LessThan lessThan_def check_keys_def)
+     apply (force simp add:keys_consistent_def forall_subtrees_def rev_apply_def keys_consistent_1_def check_keys_def key_indexes_def atLeast0LessThan lessThan_def)    
+  
+  apply (subgoal_tac "ks ~= []") prefer 2 apply (force simp add:wellformed_fts_focus_def wellformed_tree_def wf_size_def forall_subtrees_def rev_apply_def wf_size_1_def)
+  apply (case_tac a,simp)
+  apply (subgoal_tac "is_subnode ((ks, rs), index) b \<and> linked_context (lb, b, rb) list")
+  prefer 2
+  apply (case_tac "list")
+   (*list = []*)
+   apply (simp add:is_subnode_def,case_tac b,case_tac ab,force simp add:wellformed_context_1_def wellformed_fts_1_def dest_fts_state_def)
+  
+   (*list ~= []*)
+   apply simp
+   apply (case_tac b,case_tac ac,case_tac ab,simp)
+   apply (simp add:is_subnode_def,case_tac b,case_tac ab,force simp add:wellformed_context_1_def wellformed_fts_1_def dest_fts_state_def)  
+  apply (case_tac "index = 0")
+   (*index = 0*)
+   apply (force simp add:get_lower_upper_keys_for_node_t_def)
+   
+   (*index ~= 0*)
+   apply (case_tac "index = length ks")
+   apply (erule conjE)+
+   apply (force simp add:get_lower_upper_keys_for_node_t_def)
+
+   (*0 < index*)
+   apply (force simp add:get_lower_upper_keys_for_node_t_def)
 done
 end
