src/Util.thy
@@ -73,7 +73,5 @@ definition list_replace_1_at_n :: "'a list \<Rightarrow> nat \<Rightarrow> 'a \<
 
 definition list_ordered_insert :: "('a => bool) => 'a => 'a list => 'a list" where
 "list_ordered_insert is_ord e l == (
-if l = [] then [e]
-else
 (takeWhile is_ord l)@e#(tl (dropWhile is_ord l)))"
 end
